specs/Spec.Tree.fst
@@ -6,8 +6,8 @@ module U32 = FStar.UInt32
 
 open FStar.Seq
 open Lib.Seq
-open Spec.Heap
 open Yazi.Tree.Types
+include Spec.Heap
 include Spec.Tree.Lemmas
 
 /// Merge two trees that have the lowest frequencies after the call of pqremove.
@@ -19,7 +19,7 @@ let pqmerge (ts: heap_wf_ts) (node: nat): Pure tree_state_wf
   let hl = U8.v ts.depth.[il] in
   let l = ts.forest.[il] in
   let t1 = ts.tree.(il) <- ({
-    (ts.tree).[il] with
+    ts.tree.[il] with
     dad_or_len = U16.uint_to_t node;
   }) in
  
@@ -27,7 +27,7 @@ let pqmerge (ts: heap_wf_ts) (node: nat): Pure tree_state_wf
   let hr = U8.v ts.depth.[ir] in
   let r = ts.forest.[ir] in
   let t2 = t1.(ir) <- ({
-    (ts.tree).[ir] with
+    ts.tree.[ir] with
     dad_or_len = U16.uint_to_t node;
   }) in
 
@@ -55,68 +55,70 @@ let pqmerge (ts: heap_wf_ts) (node: nat): Pure tree_state_wf
     depth = ts.depth.(node) <- U8.uint_to_t dt';
     tree = t3;
   } in
+  assert(freq_corr ts 1 /\ freq_corr ts ts.heap_max);
+  assert(freq_corr ts' ts'.heap_max /\ freq_corr ts' ts.heap_max);
+  assert(freq t' == U16.v (t3.[il]).freq_or_code + U16.v (t3.[ir]).freq_or_code);
   lemma_pqmerge_main ts node ts' t';
-  admit();
   ts'
 
-#push-options "--z3refresh --z3rlimit 1024 --fuel 1 --ifuel 1"
-/// Merge the two trees that have the lowest frequencies.
-let merge_tree (ts: forest_wf_ts) (node: nat):
-  Ghost forest_wf_ts
-  (requires
-    ts.heap_len > 1 /\
-    // (forall i. i >= node ==> U8.v (ts.depth).[i] == 0) /\
-    is_max_id ts node)
-  (ensures fun ts' ->
-    ts' == {
-      ts with
-      heap = ts'.heap;
-      heap_len = ts.heap_len - 1;
-      heap_max = ts.heap_max - 2;
-      forest = ts'.forest;
-      depth = ts'.depth;
-      tree = ts'.tree;
-    } /\
-    (forall s. U32.v s <> node ==>
-      count s (element_seq ts) == count s (element_seq ts')) /\
-    count (U32.uint_to_t node) (element_seq ts') == 1 /\
-    permutation nat (forest_symbols ts) (forest_symbols ts')) =
-  let ts' = pqremove ts in
+// #push-options "--z3refresh --z3rlimit 1024 --fuel 1 --ifuel 1"
+// /// Merge the two trees that have the lowest frequencies.
+// let merge_tree (ts: forest_wf_ts) (node: nat):
+//   Ghost forest_wf_ts
+//   (requires
+//     ts.heap_len > 1 /\
+//     // (forall i. i >= node ==> U8.v (ts.depth).[i] == 0) /\
+//     is_max_id ts node)
+//   (ensures fun ts' ->
+//     ts' == {
+//       ts with
+//       heap = ts'.heap;
+//       heap_len = ts.heap_len - 1;
+//       heap_max = ts.heap_max - 2;
+//       forest = ts'.forest;
+//       depth = ts'.depth;
+//       tree = ts'.tree;
+//     } /\
+//     (forall s. U32.v s <> node ==>
+//       count s (element_seq ts) == count s (element_seq ts')) /\
+//     count (U32.uint_to_t node) (element_seq ts') == 1 /\
+//     permutation nat (forest_symbols ts) (forest_symbols ts')) =
+//   let ts' = pqremove ts in
 
-  let il = U32.v (ts'.heap).[ts'.heap_max] in
-  let hl = U8.v (ts'.depth).[il] in
-  let l = (ts'.forest).[il] in
-  let t1 = ts.tree.(il) <- ({
-    (ts.tree).[il] with
-    dad_or_len = U16.uint_to_t node;
-  }) in
+//   let il = U32.v (ts'.heap).[ts'.heap_max] in
+//   let hl = U8.v (ts'.depth).[il] in
+//   let l = (ts'.forest).[il] in
+//   let t1 = ts.tree.(il) <- ({
+//     (ts.tree).[il] with
+//     dad_or_len = U16.uint_to_t node;
+//   }) in
  
-  let ir = U32.v (ts'.heap).[1] in
-  let hr = U8.v (ts'.depth).[ir] in
-  let r = (ts'.forest).[ir] in
-  let t2 = t1.(ir) <- ({
-    (ts.tree).[ir] with
-    dad_or_len = U16.uint_to_t node;
-  }) in
+//   let ir = U32.v (ts'.heap).[1] in
+//   let hr = U8.v (ts'.depth).[ir] in
+//   let r = (ts'.forest).[ir] in
+//   let t2 = t1.(ir) <- ({
+//     (ts.tree).[ir] with
+//     dad_or_len = U16.uint_to_t node;
+//   }) in
  
-  let t' = Node l node (freq l + freq r) r in
-  let dt' = (1 + (if hl >= hr then hl else hr)) % pow2 8 in
-  let t3 = t2.(node) <- ({
-    freq_or_code = (t2.[ir]).freq_or_code `U16.add` (t2.[ir]).freq_or_code;
-    dad_or_len = U16.uint_to_t node;
-  }) in
-  admit();
-  // lemma_wf_forest_symbols_disjoint ts' ts'.heap_max 1;
+//   let t' = Node l node (freq l + freq r) r in
+//   let dt' = (1 + (if hl >= hr then hl else hr)) % pow2 8 in
+//   let t3 = t2.(node) <- ({
+//     freq_or_code = (t2.[ir]).freq_or_code `U16.add` (t2.[ir]).freq_or_code;
+//     dad_or_len = U16.uint_to_t node;
+//   }) in
+//   admit();
+//   // lemma_wf_forest_symbols_disjoint ts' ts'.heap_max 1;
 
-  let heap_max' = ts'.heap_max - 1 in
-  let heap' = upd ts'.heap heap_max' (U32.uint_to_t ir) in
+//   let heap_max' = ts'.heap_max - 1 in
+//   let heap' = upd ts'.heap heap_max' (U32.uint_to_t ir) in
  
-  let ts'' = {
-    ts' with
-    heap = heap';
-    heap_max = heap_max';
-    forest = upd ts'.forest node t';
-    depth = ts'.depth.(node) <- (U8.uint_to_t dt');
-    tree = t3;
-  } in
-  pqdownheap ts'' 1ul
+//   let ts'' = {
+//     ts' with
+//     heap = heap';
+//     heap_max = heap_max';
+//     forest = upd ts'.forest node t';
+//     depth = ts'.depth.(node) <- (U8.uint_to_t dt');
+//     tree = t3;
+//   } in
+//   pqdownheap ts'' 1ul
